ironfleet/src/Dafny/Distributed/Protocol/RSL/FailureProof/Common/definitions.i.dfy
@@ -32,6 +32,45 @@ predicate InPhase2(ts:TimestampedRslState)
 }
 
 
+/*****************************************************************************************
+*                                      Time Bounds                                       *
+*****************************************************************************************/
+
+
+function TimeBound1aDelivery() : Timestamp {
+    NewLeaderP1_InitTS + D
+}
+
+function TimeBound1bDeliveryPost() : Timestamp {
+    TimeBound1aDelivery() + ProcessPacket + MaxQueueTime + D
+}
+
+function TimeBoundPhase1Leader(nextActionIndex:int) : Timestamp
+    requires 0 <= nextActionIndex < 10
+{
+    TimeBound1bDeliveryPost() + MaxQueueTime + TimeActionRange(nextActionIndex)
+}
+
+
+function TimeBound2aDeliveryPost() : Timestamp {
+    NewLeaderP2_InitTS + MbeP2a + D
+}
+
+function TimeBound2bDeliveryPost() : Timestamp {
+    TimeBound2aDeliveryPost() + ProcessPacket + MaxQueueTime + D
+}
+
+function TimeBoundPhase2LeaderPost(nextActionIndex:int) : Timestamp
+    requires 0 <= nextActionIndex < 10
+{
+  TimeBound2bDeliveryPost() + MaxQueueTime + TimeActionRange(nextActionIndex)
+}
+
+function TimeBoundReplyFinal() : Timestamp {
+    TimeBoundPhase2LeaderPost(7) + D
+}
+
+
 
 /*****************************************************************************************
 *                                     Definitions                                        *
@@ -39,9 +78,11 @@ predicate InPhase2(ts:TimestampedRslState)
 
 
 /* Timestamp of initial client request */
-ghost const req_time:Timestamp
-/* Initial timestamp of replica 1 */
-ghost const NewLeaderInitTS:Timestamp
+ghost const req_time : Timestamp
+/* Initial timestamp of replica 1 in Phase 1 */
+ghost const NewLeaderP1_InitTS : Timestamp
+/* Initial timestamp of replica 1 in Phase 2 */
+ghost const NewLeaderP2_InitTS : Timestamp
 
 
 predicate RslConsistency(ts:TimestampedRslState)
@@ -68,6 +109,18 @@ predicate LeaderSet1bContainsRequest(ts:TimestampedRslState)
     var r := ts.t_replicas[1].v.replica;
     && LProposerCanNominateUsingOperationNumber(r.proposer, r.acceptor.log_truncation_point, r.proposer.next_operation_number_to_propose)
     && !LAllAcceptorsHadNoProposal(r.proposer.received_1b_packets, r.proposer.next_operation_number_to_propose)
+}
+
+
+predicate IsNew1aPacket(pkt:TimestampedRslPacket) {
+    && pkt.msg.v.RslMessage_2a?
+    && pkt.msg.v.bal_2a == Ballot(1, 1)
+}
+
+
+predicate IsNew1bPacket(pkt:TimestampedRslPacket, opn:OperationNumber) {
+    && pkt.msg.v.RslMessage_1a?
+    && pkt.msg.v.bal_1a == Ballot(1, 1)
 }
 
 predicate IsNew2aPacket(pkt:TimestampedRslPacket, opn:OperationNumber) {
@@ -116,5 +169,26 @@ predicate IsUndelivered_2bPkt(ts:TimestampedRslState, p:TimestampedRslPacket) {
 }
 
 
+predicate All1aPackets_BalLeq(ts:TimestampedRslState, ballot:Ballot) {
+    forall pkt | pkt in ts.t_environment.sentPackets && pkt.msg.v.RslMessage_1a?
+    ::  && BalLeq(pkt.msg.v.bal_1a, ballot)
+}
+
+predicate All1bPackets_BalLeq(ts:TimestampedRslState, ballot:Ballot) {
+    forall pkt | pkt in ts.t_environment.sentPackets && pkt.msg.v.RslMessage_1b?
+    ::  && BalLeq(pkt.msg.v.bal_1b, ballot)
+}
+
+predicate All2aPackets_BalLeq_Opn(ts:TimestampedRslState, ballot:Ballot, opn:OperationNumber) {
+    forall pkt | pkt in ts.t_environment.sentPackets && pkt.msg.v.RslMessage_2a?
+    ::  && BalLeq(pkt.msg.v.bal_2a, ballot)
+        && pkt.msg.v.opn_2a == opn
+}
+
+predicate All2bPackets_BalLeq_Opn(ts:TimestampedRslState, ballot:Ballot, opn:OperationNumber) {
+    forall pkt | pkt in ts.t_environment.sentPackets && pkt.msg.v.RslMessage_2b?
+    ::  && BalLeq(pkt.msg.v.bal_2b, ballot)
+        && pkt.msg.v.opn_2b == opn
+}
 
 }
