ironfleet/src/Dafny/Distributed/Protocol/RSL/FailureProof/Phase1/Phase1Proof.i.dfy
@@ -17,12 +17,19 @@ import opened Common_Definitions
 
 predicate P1Assumption(s:TimestampedRslState) {
     && CommonAssumptions(s)
-    && LeaderAlwaysOne(s)
-    && (var nextStep := s.t_environment.nextStep; nextStep.LEnvStepHostIos? ==>
-        (forall io :: io in nextStep.ios && io.LIoOpReceive? ==> !io.r.msg.v.RslMessage_Heartbeat?))
-    
+    && (var nextStep := ts.t_environment.nextStep; 
+        nextStep.LEnvStepHostIos? ==>
+            && (forall io | io in nextStep.ios :: !io.LIoOpTimeoutReceive?)
+            && (forall io | io in nextStep.ios && io.LIoOpReceive? :: !io.r.msg.v.RslMessage_Heartbeat? && !io.r.msg.v.RslMessage_Request? && !io.r.msg.v.RslMessage_AppStateSupply?)
+    )
+    && |ts.t_replicas| > 2 
+    && NewLeaderDoesNotReceiveOld2a2b(ts)
+    && NewLeaderDoesNotProposeFurtherOps(ts, opn)
+    && LeaderAlwaysOne(ts)
+    && minD < SelfDelivery < D < 2*minD
+    && ProcessPacket > 0
+    && SelfDelivery + TimeActionRange(0) < D
 }
-
 
 predicate LeaderAlwaysOne(s:TimestampedRslState)
     requires |s.t_replicas| > 2 
@@ -30,6 +37,12 @@ predicate LeaderAlwaysOne(s:TimestampedRslState)
     && s.t_replicas[1].v.replica.proposer.election_state.current_view == Ballot(1, 1)
     && (forall idx | 2 <= idx < |s.t_replicas| 
         :: s.t_replicas[idx].v.replica.proposer.current_state == 0)
+}
+
+predicate OldLeaderCrashed(s:TimestampedRslState, s':TimestampedRslState)
+    requires |s.t_replicas| > 2 
+{
+    forall idx, tios | TimestampedRslNextOneReplica(ps, ps', idx, ios) :: idx != 0
 }
 
 
@@ -43,21 +56,45 @@ predicate LeaderAlwaysOne(s:TimestampedRslState)
 predicate AlwaysInvariantP1(ts:TimestampedRslState, opn:OperationNumber)
     requires |ts.t_replicas| > 2
 {
+    var l := ts.t_replicas[1];
+    var r := l.v.replica;
+    && 0 <= ts.t_replicas[1].v.nextActionIndex <= 9
     && ServersAreNotClients(ts)
     && LSetOfMessage1b(ts.t_replicas[1].v.replica.proposer.received_1b_packets)
     && AlwaysInvariantP1_RequestSrcAndBatchSize(ts, opn)
+    && All1aPackets_BalLeq_Opn(ts, Ballot(1, 1))
+    && All1bPackets_BalLeq_Opn(ts, Ballot(1, 1))
+    && All2aPackets_BalLeq_Opn(ts, Ballot(1, 0), opn)
+    && All2bPackets_BalLeq_Opn(ts, Ballot(1, 0), opn)
+    && (!exists pkt :: pkt in ts.t_environment.sentPackets && IsNew2aPacket(pkt, opn))
+    && (!exists pkt :: pkt in ts.t_environment.sentPackets && IsNew2bPacket(pkt, opn))
+    && (!exists pkt :: pkt in ts.t_environment.sentPackets && IsNewReplyPacket(ts, pkt))
     && ts.t_replicas[1].v.replica.proposer.request_queue == []
     && (forall pkt | pkt in ts.undeliveredPackets :: pkt in ts.t_environment.sentPackets)
     && ts.t_replicas[1].v.replica.learner.unexecuted_learner_state == map[]
     && ts.t_replicas[1].v.replica.executor.next_op_to_execute == OutstandingOpUnknown()
-    && ts.t_replicas[1].v.replica.proposer.current_view_suspectors := {}
+    && ts.t_replicas[1].v.replica.proposer.current_view_suspectors == {}
+
+    && r.proposer.current_state == 2
+    && r.proposer.election_state.current_view == Ballot(1, 1)
+    && r.proposer.max_ballot_i_sent_1a == Ballot(1, 1)
+    && opn == r.proposer.next_operation_number_to_propose
+
+    // Learner and Executor states, maintain for phase 2
+    && opn == r.executor.ops_complete
+    && r.learner.unexecuted_learner_state == map[]
+    && r.executor.next_op_to_execute == OutstandingOpUnknown()
+    && BalLt(r.learner.max_ballot_seen, Ballot(1, 1))
 }
 
 
+/* Current identical as in P2 */
 predicate AlwaysInvariantP1_RequestSrcAndBatchSize(ts:TimestampedRslState, opn:OperationNumber)
     requires |ts.t_replicas| > 2
     requires LSetOfMessage1b(ts.t_replicas[1].v.replica.proposer.received_1b_packets)
-{
+{   
+    && All2aPackets_BalLeq_Opn(ts, Ballot(1, 0), opn)
+    && All2bPackets_BalLeq_Opn(ts, Ballot(1, 0), opn)
     && (forall pkt | IsUndelivered_2aPkt(ts, pkt) :: RequestBatchSrcInClientIds(ts, pkt.msg.v.val_2a))
     && (forall pkt | IsUndelivered_2bPkt(ts, pkt) :: RequestBatchSrcInClientIds(ts, pkt.msg.v.val_2b))
     && (forall pkt | pkt in ts.t_environment.sentPackets && pkt.msg.v.RslMessage_2a? :: |pkt.msg.v.val_2a| > 0)
@@ -67,12 +104,39 @@ predicate AlwaysInvariantP1_RequestSrcAndBatchSize(ts:TimestampedRslState, opn:O
             && RequestBatchSrcInClientIds(ts, pkt.msg.v.votes[opn'].max_val))
     && (forall v | LValIsHighestNumberedProposal(v, ts.t_replicas[1].v.replica.proposer.received_1b_packets, opn)
         :: |v| > 0)
+    // Leader's received_1b_packets
     && (forall pkt, op | pkt in ts.t_replicas[1].v.replica.proposer.received_1b_packets && pkt.msg.RslMessage_1b? && op in pkt.msg.votes
         :: RequestBatchSrcInClientIds(ts, pkt.msg.votes[op].max_val))
+    // Acceptors
     && (forall idx, opn'| 0 <= idx < |ts.t_replicas| && opn' in ts.t_replicas[idx].v.replica.acceptor.votes
         ::  && |ts.t_replicas[idx].v.replica.acceptor.votes[opn'].max_val| > 0   
             &&  RequestBatchSrcInClientIds(ts, ts.t_replicas[idx].v.replica.acceptor.votes[opn'].max_val)
     )
+}
+
+
+// Things that are true before 1a packets are sent out by the leader
+predicate Before_1a_Sent_Invariant(ts:TimestampedRslState, opn:OperationNumber) 
+    requires |ts.t_replicas| > 2
+    requires RslConsistency(ts)
+{
+    // Timestamp 
+    && TimeLe(l.ts, NewLeaderP1_InitTS)  // TODO
+    // TODO also need timestamp on 1a packets, since these are already sent
+
+    // Network
+    var l := ts.t_replicas[1];
+    var r := l.v.replica;
+    && All1aPackets_BalLeq_Opn(ts, Ballot(1, 1))
+    && All1bPackets_BalLeq_Opn(ts, Ballot(1, 0))
+    && (forall pkt :: pkt in ts.t_environment.sentPackets && pkt.msg.v.RslMessage_1a? :: IsNew1aPacket(pkt))
+    && (!exists pkt :: pkt in ts.t_environment.sentPackets && IsNew1bPacket(pkt))
+
+    // Proposer
+    && |r.proposer.received_1b_packets| < LMinQuorumSize(s.constants.all.config)
+
+    // Acceptors
+    // TODO: Need quorum of acceptors accepted only opn. Or somehow assume this?
 }
 
 
